theories/Iris/TotalWeakestPre.v
@@ -56,10 +56,10 @@ Module Type IrisTotalWeakestPre
   (Import IP   : IrisParameters B)
   (Import IR   : IrisResources B PROG SEM IPre IP).
 
-  Definition semTWP {Σ} `{sG : sailGS Σ} [Γ τ] (s : Stm Γ τ)
-    (Q : Post Γ τ) (δ : CStore Γ) : iProp Σ :=
+  Definition semTWP {Σ} `{sG : sailGS Σ} [Γ τ] (δ : CStore Γ) (s : Stm Γ τ)
+    (Q : Post Γ τ) : iProp Σ :=
     WP (MkConf s δ) [{ v, Q (valconf_val v) (valconf_store v) }].
-  Global Arguments semTWP {Σ} {sG} [Γ] [τ] s%_exp Q%_I δ.
+  Global Arguments semTWP {Σ} {sG} [Γ] [τ] δ s%_exp Q%_I.
 
   Ltac fold_semTWP :=
     first
@@ -68,13 +68,13 @@ Module Type IrisTotalWeakestPre
           (twp NotStuck top
               {| conf_stm := ?s; conf_store := ?δ |}
               (fun v => ?Q (valconf_val v) (valconf_store v)))
-        with (semTWP s Q δ)
+        with (semTWP δ s Q)
       | progress
           change_no_check
           (twp NotStuck top
               {| conf_stm := ?s; conf_store := ?δ |}
               ?Q)
-        with (semTWP s (fun v δ' => Q (MkValConf _ v δ')) δ);
+        with (semTWP δ s (fun v δ' => Q (MkValConf _ v δ')));
         try (progress (cbn [valconf_val valconf_store]))
       ].
 
@@ -84,14 +84,14 @@ Module Type IrisTotalWeakestPre
 
     Lemma semTWP_unfold [Γ τ] (s : Stm Γ τ)
       (Q : Post Γ τ) (δ : CStore Γ) :
-      semTWP s Q δ ⊣⊢
+      semTWP δ s Q ⊣⊢
         match stm_to_val s with
         | Some v => |={⊤}=> Q v δ
         | None   => ∀ (γ1 : RegStore) (μ1 : Memory),
                        regs_inv γ1 ∗ mem_inv μ1 ={⊤,∅}=∗
                        (∀ (s2 : Stm Γ τ) (δ2 : CStore Γ) (γ2 : RegStore) (μ2 : Memory),
                           ⌜⟨ γ1, μ1, δ , s ⟩ ---> ⟨ γ2, μ2, δ2, s2 ⟩⌝ ={∅}=∗
-                          |={∅,⊤}=> (regs_inv γ2 ∗ mem_inv μ2) ∗ semTWP s2 Q δ2)
+                          |={∅,⊤}=> (regs_inv γ2 ∗ mem_inv μ2) ∗ semTWP δ2 s2 Q)
         end.
     Proof.
       unfold semTWP. rewrite twp_unfold. unfold twp_pre. cbn.
@@ -121,8 +121,8 @@ Module Type IrisTotalWeakestPre
                        regs_inv γ1 ∗ mem_inv μ1 ={⊤,∅}=∗
                        (∀ (s2 : Stm Γ τ) (δ2 : CStore Γ) (γ2 : RegStore) (μ2 : Memory),
                           ⌜⟨ γ1, μ1, δ , s ⟩ ---> ⟨ γ2, μ2, δ2, s2 ⟩⌝ ={∅}=∗
-                          |={∅,⊤}=> (regs_inv γ2 ∗ mem_inv μ2) ∗ semTWP s2 Q δ2)
-        end ⊢ semTWP s Q δ.
+                          |={∅,⊤}=> (regs_inv γ2 ∗ mem_inv μ2) ∗ semTWP δ2 s2 Q)
+        end ⊢ semTWP δ s Q.
     Proof.
       rewrite semTWP_unfold.
       destruct (stm_to_val s); first easy.
@@ -135,7 +135,7 @@ Module Type IrisTotalWeakestPre
     Qed.
 
     Lemma semTWP_mono [Γ τ] (s : Stm Γ τ) (P Q : Post Γ τ) (δ : CStore Γ) :
-      ⊢ (semTWP s P δ -∗ (∀ v δ, P v δ -∗ Q v δ) -∗ semTWP s Q δ).
+      ⊢ (semTWP δ s P -∗ (∀ v δ, P v δ -∗ Q v δ) -∗ semTWP δ s Q).
     Proof.
       unfold semTWP. iIntros "WP PQ".
       iApply (twp_strong_mono with "WP"); auto.
@@ -143,16 +143,16 @@ Module Type IrisTotalWeakestPre
       by iApply "PQ".
     Qed.
     Lemma semTWP_val {Γ τ} (v : Val τ) (Q : Post Γ τ) (δ : CStore Γ) :
-      semTWP (stm_val τ v) Q δ ⊣⊢ |={⊤}=> Q (inl v) δ.
+      semTWP δ (stm_val τ v) Q ⊣⊢ |={⊤}=> Q (inl v) δ.
     Proof. rewrite semTWP_unfold. reflexivity. Qed.
 
     Lemma semTWP_fail {Γ τ s} (Q : Post Γ τ) (δ : CStore Γ) :
-      semTWP (stm_fail _ s) Q δ ⊣⊢ |={⊤}=> Q (inr s) δ.
+      semTWP δ (stm_fail _ s) Q ⊣⊢ |={⊤}=> Q (inr s) δ.
     Proof. rewrite semTWP_unfold. reflexivity. Qed.
 
     Lemma semTWP_exp {Γ τ} (e : Exp Γ τ) :
       ⊢ ∀ (Q : Post Γ τ) (δ : CStore Γ),
-          Q (inl (eval e δ)) δ -∗ semTWP (stm_exp e) Q δ.
+          Q (inl (eval e δ)) δ -∗ semTWP δ (stm_exp e) Q.
     Proof.
       iIntros (Q δ1) "P". rewrite <-semTWP_unfold_nolc. cbn.
       iIntros (γ1 μ1) "state_inv".
@@ -164,8 +164,8 @@ Module Type IrisTotalWeakestPre
 
     Lemma semTWP_block {Γ τ Δ} (δΔ : CStore Δ) (s : Stm (Γ ▻▻ Δ) τ) :
       ⊢ ∀ (Q : Post Γ τ) (δ : CStore Γ),
-          semTWP s (fun v δ1 => Q v (env.drop Δ δ1)) (δ ►► δΔ) -∗
-          semTWP (stm_block δΔ s) Q δ.
+          semTWP (δ ►► δΔ) s (fun v δ1 => Q v (env.drop Δ δ1)) -∗
+          semTWP δ (stm_block δΔ s) Q.
     Proof.
       iIntros (Q δ) "H". rewrite /semTWP.
       iAssert (∃ Φ, ∀ v, Φ v ∗-∗ Q (valconf_val v) (env.drop Δ (valconf_store v)))%I as "(%Φ & HΦ)".
@@ -201,8 +201,8 @@ Module Type IrisTotalWeakestPre
 
     Lemma semTWP_call_frame {Γ τ Δ} (δΔ : CStore Δ) (s : Stm Δ τ) :
       ⊢ ∀ (Q : Post Γ τ) (δ : CStore Γ),
-          semTWP s (fun v _ => Q v δ) δΔ -∗
-          semTWP (stm_call_frame δΔ s) Q δ.
+          semTWP δΔ s (fun v _ => Q v δ) -∗
+          semTWP δ (stm_call_frame δΔ s) Q.
     Proof.
       iIntros (Q δ) "H". rewrite /semTWP.
       iAssert (∃ Φ, ∀ v, Φ v ∗-∗ Q (valconf_val v) δ)%I as "(%Φ & HΦ)".
@@ -232,8 +232,8 @@ Module Type IrisTotalWeakestPre
 
     Lemma semTWP_call_inline {Γ τ Δ} (f : 𝑭 Δ τ) (es : NamedEnv (Exp Γ) Δ) :
       ⊢ ∀ (Q : Post Γ τ) (δΓ : CStore Γ),
-          semTWP (FunDef f) (fun vτ _ => Q vτ δΓ) (evals es δΓ) -∗
-          semTWP (stm_call f es) Q δΓ.
+          semTWP (evals es δΓ) (FunDef f) (fun vτ _ => Q vτ δΓ) -∗
+          semTWP δΓ (stm_call f es) Q.
     Proof.
       iIntros (Q δΓ) "wpbody". rewrite <-(semTWP_unfold_nolc (stm_call f es)). cbn.
       iIntros (γ1 μ1) "state_inv".
@@ -245,7 +245,7 @@ Module Type IrisTotalWeakestPre
 
     Lemma semTWP_bind {Γ τ σ} (s : Stm Γ σ) (k : Val σ → Stm Γ τ) :
       ⊢ ∀ (Q : Post Γ τ) (δ : CStore Γ),
-          semTWP s (fun v => semTWP (lift_cnt k v) Q) δ -∗ semTWP (stm_bind s k) Q δ.
+          semTWP δ s (fun v δ => semTWP δ (lift_cnt k v) Q) -∗ semTWP δ (stm_bind s k) Q.
     Proof.
       iIntros (Q δ) "H". rewrite /semTWP.
       iAssert (∃ Φ, ∀ v, Φ v ∗-∗ WP (MkConf (lift_cnt k (valconf_val v)) (valconf_store v))
@@ -282,11 +282,11 @@ Module Type IrisTotalWeakestPre
 
     Lemma semTWP_let {Γ τ x σ} (s : Stm Γ σ) (k : Stm (Γ ▻ x∷σ) τ) :
       ⊢ ∀ (Q : Post Γ τ) (δ : CStore Γ),
-          semTWP s (fun v1 δ1 => match v1 with
-                                | inl v1 => semTWP k (fun v2 δ2 => Q v2 (env.tail δ2)) δ1.[x∷σ ↦ v1]
-                                | inr m1 => semTWP (of_ival (inr m1)) Q δ1
-                                end) δ -∗
-          semTWP (let: x ∷ σ := s in k) Q δ.
+          semTWP δ s (fun v1 δ1 => match v1 with
+                                | inl v1 => semTWP δ1.[x∷σ ↦ v1] k (fun v2 δ2 => Q v2 (env.tail δ2))
+                                | inr m1 => semTWP δ1 (of_ival (inr m1)) Q
+                                end) -∗
+          semTWP δ (let: x ∷ σ := s in k) Q.
     Proof.
       iIntros (Q δΓ) "WPs". rewrite <-(semTWP_unfold_nolc (stm_let x σ s k)). cbn.
       iIntros (γ1 μ1) "state_inv".
@@ -301,10 +301,10 @@ Module Type IrisTotalWeakestPre
 
     Lemma semTWP_seq {Γ τ σ} (s : Stm Γ σ) (k : Stm Γ τ) :
       ⊢ ∀ (Q : Post Γ τ) (δ : CStore Γ),
-          semTWP s (λ v δ, match v with
-                          | inl _ => semTWP k Q δ
-                          | inr m => semTWP (of_ival (inr m)) Q δ
-                          end) δ -∗ semTWP (s;;k) Q δ.
+          semTWP δ s (λ v δ, match v with
+                          | inl _ => semTWP δ k Q
+                          | inr m => semTWP δ (of_ival (inr m)) Q
+                          end) -∗ semTWP δ (s;;k) Q.
     Proof.
       iIntros (Q δ) "WPs". rewrite <-(semTWP_unfold_nolc (stm_seq s k)). cbn.
       iIntros (γ1 μ1) "state_inv".
@@ -318,9 +318,9 @@ Module Type IrisTotalWeakestPre
 
     Lemma semTWP_assertk {Γ τ} (e1 : Exp Γ ty.bool) (e2 : Exp Γ ty.string) (k : Stm Γ τ) :
       ⊢ ∀ (Q : Post Γ τ) (δ : CStore Γ),
-          (⌜eval e1 δ = true⌝ → semTWP k Q δ) -∗
-          (⌜eval e1 δ = false⌝ → semTWP (fail (eval e2 δ)) Q δ) -∗
-          semTWP (stm_assertk e1 e2 k) Q δ.
+          (⌜eval e1 δ = true⌝ → semTWP δ k Q) -∗
+          (⌜eval e1 δ = false⌝ → semTWP δ (fail (eval e2 δ)) Q) -∗
+          semTWP δ (stm_assertk e1 e2 k) Q.
     Proof.
       iIntros (Q δ) "WPtrue WPfalse". rewrite <-(semTWP_unfold_nolc (stm_assertk e1 e2 k)). cbn.
       iIntros (γ1 μ1) "state_inv".
@@ -333,7 +333,7 @@ Module Type IrisTotalWeakestPre
     Lemma semTWP_read_register {Γ τ} (reg : 𝑹𝑬𝑮 τ) :
       ⊢ ∀ (Q : Post Γ τ) (δ : CStore Γ),
           (∃ v : Val τ, reg_pointsTo reg v ∗ (reg_pointsTo reg v -∗ Q (inl v) δ)) -∗
-          semTWP (stm_read_register reg) Q δ.
+          semTWP δ (stm_read_register reg) Q.
     Proof.
       iIntros (Q δ) "[% [Hreg HP]]". rewrite <-semTWP_unfold_nolc. cbn.
       iIntros (γ1 μ1) "[Hregs Hmem]".
@@ -347,7 +347,7 @@ Module Type IrisTotalWeakestPre
     Lemma semTWP_write_register {Γ τ} (reg : 𝑹𝑬𝑮 τ) (e : Exp Γ τ) :
       ⊢ ∀ (Q : Post Γ τ) (δ : CStore Γ),
           (∃ v : Val τ, reg_pointsTo reg v ∗ (reg_pointsTo reg (eval e δ) -∗ Q (inl (eval e δ)) δ)) -∗
-          semTWP (stm_write_register reg e) Q δ.
+          semTWP δ (stm_write_register reg e) Q.
     Proof.
       iIntros (Q δ) "[% [Hreg HP]]". rewrite <-semTWP_unfold_nolc. cbn.
       iIntros (γ1 μ1) "[Hregs Hmem]".
@@ -360,11 +360,11 @@ Module Type IrisTotalWeakestPre
 
     Lemma semTWP_assign {Γ τ x} (xInΓ : x∷τ ∈ Γ) (s : Stm Γ τ) :
       ⊢ ∀ (Q : Post Γ τ) (δ : CStore Γ),
-          semTWP s (λ (a : IVal τ) (δ0 : CStore Γ), match a with
+          semTWP δ s (λ (a : IVal τ) (δ0 : CStore Γ), match a with
                                                    | inl a => Q (inl a) (δ0 ⟪ x ↦ a ⟫)
                                                    | inr m => Q (inr m) δ0
-                                                   end) δ -∗
-          semTWP (stm_assign x s) Q δ.
+                                                   end) -∗
+          semTWP δ (stm_assign x s) Q.
     Proof.
       iIntros (Q δ) "H". rewrite /semTWP.
       iAssert (∃ Φ, ∀ v, Φ v ∗-∗ 
@@ -406,21 +406,20 @@ Module Type IrisTotalWeakestPre
     Lemma semTWP_pattern_match {Γ τ σ} (s : Stm Γ σ) (pat : Pattern σ)
       (rhs : ∀ pc : PatternCase pat, Stm (Γ ▻▻ PatternCaseCtx pc) τ) :
       ⊢ ∀ (Q : Post Γ τ) (δ : CStore Γ),
-      semTWP s
+      semTWP δ s
         (fun vσ δ1 =>
            match vσ with
            | inl vσ =>
                let (pc,δpc) := pattern_match_val pat vσ in
-               semTWP (rhs pc)
+               semTWP (δ1 ►► δpc) (rhs pc)
                  (fun vτ δ2 =>
                     match vτ with
                     | inl vτ => Q (inl vτ) (env.drop (PatternCaseCtx pc) δ2)
                     | inr m  => Q (inr m) (env.drop (PatternCaseCtx pc) δ2)
                     end)
-                 (δ1 ►► δpc)
            | inr m => |={⊤}=> Q (inr m) δ1
-           end) δ -∗
-      semTWP (stm_pattern_match s pat rhs) Q δ.
+           end) -∗
+      semTWP δ (stm_pattern_match s pat rhs) Q.
     Proof.
       iIntros (Q δΓ) "WPs". rewrite <-(semTWP_unfold_nolc (stm_pattern_match s pat rhs)). cbn.
       iIntros (γ1 μ1) "state_inv".
@@ -441,10 +440,10 @@ Module Type IrisTotalWeakestPre
           ⌜ ForeignCall f (evals es δ) res γ γ' μ μ' ⌝
            -∗
            |={∅,⊤}=> (regs_inv γ' ∗ mem_inv μ') ∗
-                      semTWP (match res with inr v => stm_val _ v
+                      semTWP δ (match res with inr v => stm_val _ v
                                        | inl s => stm_fail _ s
-                             end) Q δ)) -∗
-        semTWP (stm_foreign f es) Q δ.
+                             end) Q)) -∗
+        semTWP δ (stm_foreign f es) Q.
     Proof.
       iIntros "H". rewrite <-semTWP_unfold_nolc. cbn. iIntros (γ1 μ1) "state_inv".
       iMod ("H" $! γ1 μ1 with "[$]") as "H". iModIntro.
@@ -452,7 +451,7 @@ Module Type IrisTotalWeakestPre
     Qed.
 
     Lemma semTWP_debugk {Γ τ} (s : Stm Γ τ) :
-      ⊢ ∀ Q δ, semTWP s Q δ -∗ semTWP (stm_debugk s) Q δ.
+      ⊢ ∀ Q δ, semTWP δ s Q -∗ semTWP δ (stm_debugk s) Q.
     Proof.
       iIntros (Q δ) "WPs". rewrite <-(semTWP_unfold_nolc (stm_debugk s)). cbn.
       iIntros (γ1 μ1) "state_inv".
@@ -462,7 +461,7 @@ Module Type IrisTotalWeakestPre
     Qed.
 
     Lemma semTWP_lemmak {Γ τ} {Δ} (l : 𝑳 Δ) (es : NamedEnv (Exp Γ) Δ) (s : Stm Γ τ) :
-      ⊢ ∀ Q δ, semTWP s Q δ -∗ semTWP (stm_lemmak l es s) Q δ.
+      ⊢ ∀ Q δ, semTWP δ s Q -∗ semTWP δ (stm_lemmak l es s) Q.
     Proof.
       iIntros (Q δ) "WPs". rewrite <-(semTWP_unfold_nolc (stm_lemmak l es s)). cbn.
       iIntros (γ1 μ1) "state_inv".
@@ -476,7 +475,7 @@ Module Type IrisTotalWeakestPre
     Lemma semTWP_Steps {Γ τ} {s1 : Stm Γ τ} {Q δ1} :
       ∀ {γ1 : RegStore} {μ1 : Memory},
         regs_inv γ1 ∗ mem_inv μ1 -∗
-        semTWP s1 Q δ1 ={⊤}=∗
+        semTWP δ1 s1 Q ={⊤}=∗
         ∃ γ2 μ2 δ2 s2 v, ⌜⟨ γ1, μ1, δ1, s1 ⟩ --->* ⟨ γ2, μ2, δ2, s2 ⟩ ⌝
                         ∗ ⌜stm_to_val s2 = Some v⌝
                         ∗ regs_inv γ2 ∗ mem_inv μ2 ∗ Q v δ2.
@@ -523,15 +522,15 @@ Module Type IrisTotalWeakestPre
   Module twptactics.
     Ltac kEval :=
       match goal with
-      | |- environments.envs_entails ?ctx (semTWP ?s ?post ?store) =>
+      | |- environments.envs_entails ?ctx (semTWP ?store ?s ?post) =>
           let s' := eval compute - [Val] in s in
           let store' := eval compute - [Val] in store in
-          change_no_check (environments.envs_entails ctx (semTWP s' post store'))
+          change_no_check (environments.envs_entails ctx (semTWP store' s' post))
       end.
 
     Ltac kStep :=
       match goal with
-      | |- environments.envs_entails ?ctx (semTWP ?stm ?post ?store) =>
+      | |- environments.envs_entails ?ctx (semTWP ?store ?stm ?post) =>
           match stm with
           | stm_val ?τ ?v => iApply semTWP_val
           | stm_exp ?e => iApply (semTWP_exp e)
