case_study/RiscvPmp/IrisModel.v
@@ -83,7 +83,7 @@ Module RiscvPmpIrisBase <: IrisBase RiscvPmpBase RiscvPmpProgram RiscvPmpSemanti
   Import iris.program_logic.weakestpre.
 
   Definition WP_loop `{sg : sailGS Σ} : iProp Σ :=
-    semWP (FunDef loop) (fun _ _ => True%I) env.nil.
+    semWP env.nil (FunDef loop) (fun _ _ => True%I).
 
   (* Useful instance for some of the Iris proofs *)
   #[export] Instance state_inhabited : Inhabited State.
